theories/Semantics.v
@@ -27,13 +27,14 @@ Inductive Step : env -> term -> term -> prefix -> Prop :=
       Step n (e1; e2) e2' (PfxCatBoth p1 p2)
   | S_Par_L : forall n x y z e e' p1 p2 p',
       MapsTo (PfxParPair p1 p2) z n ->
-      Step (subst x p1 (subst y p2 n)) e e' p' ->
+      Step (union n (union (singleton_env x p1) (singleton_env y p2))) e e' p' ->
       Step n (TmLetPar x y z e) (TmLetPar x y z e') p'
   | S_Cat_L_1 : forall t n x y z e e' p p',
       MapsTo (PfxCatFst p) z n ->
       Step (subst x p (subst y (emp t) n)) e e' p' ->
       Step n (TmLetCat t x y z e) (TmLetCat t x y z e') p'
   .
+(* TODO: FINISH DEFINITION *)
 
 Print Step.
 
