theories/Ident.v
@@ -5,10 +5,23 @@ From Coq Require Import
 
 Definition ident : Set := string.
 
+From Hammer Require Import Tactics.
+
 Bind Scope string_scope with ident.
 
 Definition eq_id : ident -> ident -> bool := eqb.
 Notation "a '=i' b" := (eq_id a b) (at level 98).
+
+Theorem eq_id_refl : forall x, (x =i x) = true.
+Proof.
+hauto lq: on use:eqb_refl.
+Qed.
+
+Theorem eq_id_notrefl : forall x y, x <> y -> (x =i y) = false.
+Proof.
+sfirstorder use:eqb_neq.
+Qed.
+
 
 Instance EqDec : EqDec Ident.ident eq :=
 {
