theories/SemSound.v
@@ -5,16 +5,36 @@ From LambdaST Require Import
     Prefix
     Environment
     Hole
+    FV
     Context.
 Require Import Coq.Program.Equality.
 
 From Hammer Require Import Tactics.
 
+Theorem maximalpush : forall e e' eta p,
+  Step eta e e' p ->
+  MaximalOn (fv e) eta ->
+  Maximal p.
+Proof.
+  intros.
+  generalize dependent H0.
+  induction H; intros.
+  - sauto lq: on.
+  - sauto lq: on.
+  - qauto l: on.
+  - sauto lq: on.
+  - sauto lq: on.
+  - sauto lq: on.
+  - admit.
+  - admit.
+Admitted.
+
+
 
 Theorem soundout : forall G e e' s eta p,
     Typed G e s ->
     Step eta e e' p ->
-    wf e ->
+    wf (fv G) e ->
     wf_ctx G ->
     EnvTyped eta G ->
     PfxTyped p s
@@ -25,17 +45,39 @@ Proof.
     generalize dependent eta.
     generalize dependent p.
     induction Hty; intros p eta e0' Hstep Hwfe HwfG Heta.
-    - sauto lq: on rew: off.
-    - sinvert Hwfe; sinvert Hstep; eapply IHHty.
+    - sinvert Hwfe. cbn in *. sauto q: on.
+    - sinvert Hwfe; sinvert Hstep.
+      assert (~fv G x) by sfirstorder use:fv_fill.
+      assert (~fv G y) by sfirstorder use:fv_fill.
+      assert (PfxTyped (PfxParPair p1 p2) (Types.TyPar s t)) by qauto l:on use: maps_to_has_type.
+      sinvert H1.
+      eapply IHHty.
       + eauto.
-      + eauto.
-      + admit.
-      + admit.
+      + eapply wf_iff; [| eauto]. intro. admit. (* i think we can do this. *)
+      + apply wf_fill in HwfG. destruct HwfG as [A [B C]].
+        apply wf_fill.
+        (* here, we need to know that x and y are not free in G.*)
+        split; try split. sfirstorder. sauto l: on. cbn in *. sfirstorder use:fv_fill.
+      + eapply fill_replace; [|eauto| |]. admit.
+        * eapply envtyped_comma; [| eapply envtyped_singleton; eauto | eapply envtyped_singleton; eauto]. admit.
+        * admit. 
+    - sinvert Hwfe; sinvert HwfG; sinvert Heta. sinvert Hstep; admit.
     - sinvert Hwfe. admit.
     - sinvert Hwfe. admit.
     - sinvert Hwfe. admit.
-    - sinvert Hwfe. admit.
-    - sinvert Hwfe. admit.
-    - admit.
-    - admit.
+    - sinvert Hwfe. apply wf_fill in HwfG. 
+      destruct HwfG as [U []]. sinvert H. apply fv_fill in H1.
+      sauto use: maps_to_has_type.
+    - sfirstorder.
+    - sinvert Hstep.
 Admitted.
+
+(*
+
+(x : s, y : s) |- fix(x:s,y:s). rec(x+1,x) : s
+|->
+cut x = x+1 in y = x in rec(x+1,x)
+WRONG!!
+
+We need a real multicut for unfolding recursive calls.
+*)
